src/3d/GenMakefile.fst
@@ -1,0 +1,137 @@
+module GenMakefile
+
+type rule_t = {
+  from: list string;
+  to: list string;
+  args: string;
+}
+
+let output_dir = "$(EVERPARSE_OUTPUT_DIR)"
+
+let print_gnu_make_rule
+  (r: rule_t)
+: Tot string
+= (* NOTE: I could use multiple target rule &: from https://www.gnu.org/software/make/manual/html_node/Multiple-Targets.html,
+     but that feature is too recent (GNU Make 4.3, February 2020)
+   *)
+  match r.to with
+  | [] -> ""
+  | a :: q ->
+    let rule = Printf.sprintf "%s : %s\n" a (String.concat " " r.from) in
+    let rule = Printf.sprintf "%s\t$(EVERPARSE_CMD) --odir %s %s\n\n" rule output_dir r.args in
+    let rule = List.Tot.fold_left (fun rule ne -> Printf.sprintf "%s%s: %s\n\ttest -f $@ && touch $@\n\n" rule ne a) rule q in
+    rule
+
+let mk_filename
+  (modul: string)
+  (ext: string)
+: Tot string
+= (Printf.sprintf "%s.%s" modul ext)
+
+let produce_types_checked_rule
+  (g: Deps.dep_graph)
+  (modul: string)
+: Tot rule_t
+= let types_fst = mk_filename modul "Types.fst" in 
+  {
+    from = types_fst :: List.Tot.map (fun m -> mk_filename m "Types.fst.checked") (Deps.dependencies g modul);
+    to = [mk_filename modul "Types.fst.checked"];
+    args = Printf.sprintf "--__micro_step verify %s" types_fst;
+  }
+
+let produce_fsti_checked_rule
+  (g: Deps.dep_graph)
+  (modul: string)
+: Tot rule_t
+= let fsti = mk_filename modul "fsti" in
+  {
+    from = fsti :: mk_filename modul "Types.fst.checked" :: List.Tot.map (fun m -> mk_filename m "fsti.checked") (Deps.dependencies g modul);
+    to = [mk_filename modul "fsti.checked"];
+    args = Printf.sprintf "--__micro_step verify %s" fsti;
+  }
+
+let produce_fst_checked_rule
+  (g: Deps.dep_graph)
+  (modul: string)
+: Tot rule_t
+= let fst = mk_filename modul "fst" in
+  {
+    from = fst :: mk_filename modul "fsti.checked" :: List.Tot.map (fun m -> mk_filename m "fsti.checked") (Deps.dependencies g modul);
+    to = [mk_filename modul "fst.checked"];
+    args = Printf.sprintf "--__micro_step verify %s" fst;
+  }
+
+let produce_types_krml_rule
+  (g: Deps.dep_graph)
+  (modul: string)
+: Tot rule_t
+=
+  {
+    from = mk_filename modul "Types.fst.checked" :: List.Tot.map (fun m -> mk_filename m "Types.fst.checked") (Deps.dependencies g modul);
+    to = [mk_filename (Printf.sprintf "%s_Types" modul) "krml"];
+    args = Printf.sprintf "--__micro_step extract %s" (mk_filename modul "Types.fst");
+  }
+
+let produce_krml_rule
+  (g: Deps.dep_graph)
+  (modul: string)
+: Tot rule_t
+=
+  {
+    from = mk_filename modul "fst.checked" :: List.Tot.map (fun m -> mk_filename m "fst.checked") (Deps.dependencies g modul);
+    to = [mk_filename modul "krml"];
+    args = Printf.sprintf "--__micro_step extract %s" (mk_filename modul "fst");
+  }
+
+let produce_fst_rule
+  (all_files: list string)
+: FStar.All.ML rule_t
+=
+  {
+    from = all_files;
+    to =
+      begin
+        let types = List.map (fun f -> mk_filename (Options.get_module_name f) "Types.fst") all_files in
+        let fsti = List.map (fun f -> mk_filename (Options.get_module_name f) "fsti") all_files in
+        let fst = List.map (fun f -> mk_filename (Options.get_module_name f) "fst") all_files in
+        types `List.Tot.append` fsti `List.Tot.append` fst
+      end;
+    args = Printf.sprintf "--__skip_deps --no_batch %s" (String.concat " " all_files);
+  }
+
+let produce_h_rule
+  (all_files: list string)
+: FStar.All.ML rule_t
+=
+  {
+    from =
+      List.map (fun f -> mk_filename (Options.get_module_name f) "krml") all_files `List.Tot.append`
+      List.map (fun f -> mk_filename (Printf.sprintf "%s_Types" (Options.get_module_name f)) "krml") all_files
+      ;
+    to = List.map (fun f -> mk_filename (Options.get_module_name f) "h") all_files;
+    args = Printf.sprintf "--__skip_deps --__produce_c_from_existing_krml %s" (String.concat " " all_files);
+  }
+
+let produce_makefile
+  (files: list string)
+: FStar.All.ML (list rule_t)
+=
+  let g = Deps.build_dep_graph_from_list files in
+  let all_files = Deps.collect_and_sort_dependencies_from_graph g files in
+  let all_modules = List.map Options.get_module_name all_files in
+  produce_h_rule all_files ::
+  produce_fst_rule all_files ::
+  List.Tot.map (produce_types_checked_rule g) all_modules `List.Tot.append`
+  List.Tot.map (produce_fsti_checked_rule g) all_modules `List.Tot.append`
+  List.Tot.map (produce_fst_checked_rule g) all_modules `List.Tot.append`
+  List.Tot.map (produce_types_krml_rule g) all_modules `List.Tot.append`
+  List.Tot.map (produce_krml_rule g) all_modules
+
+let write_gnu_makefile
+  (files: list string)
+: FStar.All.ML unit
+=
+  let makefile = Options.get_makefile_name () in
+  let file = FStar.IO.open_write_file makefile in
+  FStar.IO.write_string file (String.concat "" (List.Tot.map print_gnu_make_rule (produce_makefile files)));
+  FStar.IO.close_write_file file
