src/3d/GenMakefile.fsti
@@ -1,0 +1,5 @@
+module GenMakefile
+
+val write_gnu_makefile
+  (files: list string)
+: FStar.All.ML unit
