src/3d/Options.fsti
@@ -4,6 +4,8 @@ open FStar.All
 
 val display_usage : unit -> ML unit
 
+val compute_options (ignore: list string) : ML string
+
 val parse_cmd_line : unit -> ML (list string)
 
 val get_file_name (mname:string) : ML string
@@ -41,3 +43,9 @@ val get_equate_types_list : unit -> ML (list (string & string))
 val get_micro_step : unit -> ML (option micro_step_t)
 
 val get_produce_c_from_existing_krml : unit -> ML bool
+
+val get_skip_deps : unit -> ML bool
+
+val get_gnu_makefile : unit -> ML bool
+
+val get_makefile_name : unit -> ML string
